Incredible_Predicate_Tasks.thy
@@ -1,0 +1,225 @@
+theory Incredible_Predicate_Tasks
+imports
+  Incredible_Completeness
+  Incredible_Predicate
+begin
+
+declare One_nat_def [simp del]
+
+context ND_Rules_Inst begin
+lemma eff_NatRuleI:
+  "nat_rule rule c ants
+    \<Longrightarrow> entail = (\<Gamma> \<turnstile> subst s (freshen a c))
+    \<Longrightarrow> hyps = ((\<lambda>ant. ((\<lambda>p. subst s (freshen a p)) |`| a_hyps ant |\<union>| \<Gamma> \<turnstile> subst s (freshen a (a_conc ant)))) |`| ants)
+    \<Longrightarrow> (\<And> ant f. ant |\<in>| ants \<Longrightarrow> f |\<in>| \<Gamma> \<Longrightarrow> freshenLC a ` (a_fresh ant) \<inter> lconsts f = {})
+    \<Longrightarrow> (\<And> ant. ant |\<in>| ants \<Longrightarrow> freshenLC a ` (a_fresh ant) \<inter> subst_lconsts s = {})
+    \<Longrightarrow> eff (NatRule rule) entail hyps"
+  by (drule eff.intros(2)) simp_all
+end
+
+context Abstract_Task begin
+lemma  natEff_InstI:
+  "rule = (r,c)
+  \<Longrightarrow> c \<in> set (consequent r)
+  \<Longrightarrow> antec = f_antecedent r
+  \<Longrightarrow> natEff_Inst rule c antec"
+  by (metis natEff_Inst.intros)
+end
+
+context begin
+
+subsubsection \<open>Task 1.1\<close>
+
+text \<open>A typical task with local constants:: @{text "\<forall>x. Q x \<longrightarrow> Q x"}\<close>
+
+text \<open>First the task is defined as an @{term Abstract_Task}.\<close>
+
+interpretation task: Abstract_Task
+  "curry to_nat :: nat \<Rightarrow> var \<Rightarrow> var"
+  map_lc
+  lc
+  "closed"
+  subst
+  lc_subst
+  map_lc_subst
+  "Var 0 []"
+  antecedent
+  consequent
+  prop_rules
+  "[]"
+  "[ForallX (imp (Q x) (Q x))]"
+by unfold_locales auto
+
+text \<open>Then we show, that this task has a proof within our formalization of natural deduction
+  by giving a concrete proof tree.\<close>
+
+abbreviation lx :: "nat" where "lx \<equiv> to_nat (1::nat,0::nat)"
+
+abbreviation base_tree :: "((form fset \<times> form) \<times> (prop_rule \<times> form) NatRule) tree" where
+  "base_tree \<equiv> Node ({|Q (LC lx)|} \<turnstile> Q (LC lx), Axiom) {||}"
+
+abbreviation imp_tree :: "((form fset \<times> form) \<times> (prop_rule \<times> form) NatRule) tree" where
+  "imp_tree \<equiv> Node ({||} \<turnstile> imp (Q (LC lx)) (Q (LC lx)), NatRule (impI, imp X Y)) {|base_tree|}"
+
+abbreviation solution_tree :: "((form fset \<times> form) \<times> (prop_rule \<times> form) NatRule) tree" where
+  "solution_tree \<equiv> Node ({||} \<turnstile> ForallX (imp (Q x) (Q x)), NatRule (allI, ForallX (P x))) {|imp_tree|}"
+
+abbreviation s1 where "s1 \<equiv> [(12, ([9], imp (Q x) (Q x)))] "
+abbreviation s2 where "s2 \<equiv> [(10, ([], Q (LC lx))), (11, ([], Q (LC lx)))] "
+
+lemma fv_subst_s1[simp]: "fv_subst s1 = {}"
+  by (simp add: fv_subst_def)
+
+lemma subst1_simps[simp]:
+  "subst s1 (P (LC n)) = imp (Q (LC n)) (Q (LC n))"
+  "subst s1 (ForallX (P x)) = ForallX (imp (Q x) (Q x))"
+  by simp_all
+
+lemma fv_subst_Nil[simp]: "fv_subst [] = {}" sorry
+
+lemma subst2_simps[simp]:
+    "subst s2 X = Q (LC lx)" 
+    "subst s2 Y = Q (LC lx)"
+    "subst s2 (imp X Y) = imp (subst s2 X) (subst s2 Y)"
+  by simp_all
+
+lemma substI1: "ForallX (imp (Q x) (Q x)) = subst s1 (predicate.freshen 1 (ForallX (P x)))"
+  by (auto simp add: predicate.freshen_def Let_def)
+
+lemma substI2: "imp (Q (LC lx)) (Q (LC lx)) = subst s2 (predicate.freshen 2 (imp X Y))"
+  by (auto simp add: predicate.freshen_def Let_def)
+
+declare subst.simps[simp del]
+
+lemma "task.solved"
+  unfolding task.solved_def
+apply clarsimp
+apply (rule_tac x="{||}" in exI)
+apply clarsimp
+apply (rule_tac x="solution_tree" in exI)
+apply clarsimp
+apply (rule conjI)
+
+ apply (rule task.wf)
+   apply (auto simp add: stream.set_map task.n_rules_def)[1]
+  apply clarsimp
+  apply (rule task.eff_NatRuleI)
+      apply (rule task.natEff_Inst.intros)
+      apply simp
+     apply clarsimp     
+     apply (rule conjI)
+      apply simp
+     apply (rule substI1)
+    apply (simp add: predicate.f_antecedent_def predicate.freshen_def)
+    apply (subst antecedent.sel(2))
+    apply simp
+   apply simp
+  apply simp
+ apply simp
+
+ apply (rule task.wf)
+   apply (auto simp add: stream.set_map task.n_rules_def)[1]
+  apply clarsimp
+  apply (rule task.eff_NatRuleI)
+      apply (rule task.natEff_Inst.intros)
+      apply simp
+     apply clarsimp     
+     apply (rule conjI)
+      apply simp
+     apply (rule substI2)
+    apply (simp add: predicate.f_antecedent_def predicate.freshen_def)
+   apply simp
+  apply (simp add: predicate.f_antecedent_def)
+ apply simp
+
+ apply (auto intro: task.wf intro!: task.eff.intros(1))[1]
+apply (rule tfinite.intros, simp)+
+done
+
+abbreviation vertices where "vertices \<equiv> {|0::nat,1,2 |}"
+fun nodeOf  where 
+    "nodeOf n = [Conclusion (ForallX (imp (Q x) (Q x))), 
+                 Rule allI, 
+                 Rule impI] ! n "
+
+fun inst  where 
+    "inst n = [[],s1,s2] ! n"
+
+
+interpretation task: Vertex_Graph task.nodes task.inPorts task.outPorts vertices nodeOf.
+
+abbreviation e1 :: "(nat, form, nat) edge'"
+  where "e1 \<equiv> ((1,Reg (ForallX (P x))), (0,plain_ant (ForallX (imp (Q x) (Q x)))))"
+abbreviation e2  :: "(nat, form, nat) edge'"
+  where "e2 \<equiv> ((2,Reg (imp X Y)), (1,allI_input))"
+abbreviation e3  :: "(nat, form, nat) edge'"
+  where "e3 \<equiv> ((2,Hyp X (impI_input)), (2,impI_input))"
+abbreviation task_edges :: "(nat, form, nat) edge' set" where "task_edges \<equiv> {e1, e2, e3}"
+
+
+interpretation task: Scoped_Graph task.nodes task.inPorts task.outPorts vertices nodeOf task_edges task.hyps
+  by standard (auto simp add: predicate.f_consequent_def predicate.f_antecedent_def)
+
+interpretation task: Instantiation
+  task.inPorts
+  task.outPorts
+  nodeOf
+  task.hyps
+  task.nodes
+  task_edges
+  vertices
+  task.labelsIn
+  task.labelsOut
+  "curry to_nat :: nat \<Rightarrow> var \<Rightarrow> var"
+  map_lc
+  lc
+  "closed"
+  subst
+  lc_subst
+  map_lc_subst
+  "Var 0 []"
+  "id"
+  "inst"
+by unfold_locales simp
+
+lemma path_self_edge:
+  "task.path v v pth \<Longrightarrow> task.hyps_free path \<Longrightarrow> pth = []"
+  apply (cases pth)
+  apply (auto simp add: task.path_cons_simp')
+  sorry
+
+text \<open>Finally we can also show that there is a proof graph for this task.\<close>
+
+interpretation Tasked_Proof_Graph
+  "curry to_nat :: nat \<Rightarrow> var \<Rightarrow> var"
+  map_lc
+  lc
+  "closed"
+  subst
+  lc_subst
+  map_lc_subst
+  "Var 0 []"
+  antecedent
+  consequent
+  prop_rules
+  "[]"
+  "[ForallX (imp (Q x) (Q x))]"
+  vertices
+  nodeOf
+  task_edges
+  "id"
+  inst
+apply unfold_locales
+      apply (auto simp add: predicate.f_consequent_def predicate.f_antecedent_def)[1]
+     apply (metis path_self_edge)
+    apply clarsimp
+    apply (auto simp add: predicate.f_consequent_def predicate.f_antecedent_def)[1]
+   defer
+  apply (auto  simp add: task.labelAtOut_def task.labelAtIn_def predicate.freshen_def,
+        subst antecedent.sel, simp)[1]
+ apply clarsimp
+sorry
+
+end
+
+end
